This problem asks us to use the Regula Falsi method (also known as the False Position method) to solve the equation x² - x - 2 = 0 with initial guesses [1, 3] for three iterations. Let's break this down step-by-step:

Our function is f(x) = x² - x - 2
Initial guesses: a = 1, b = 3
We'll perform 3 iterations:

Iteration 1:
f(a) = f(1) = 1² - 1 - 2 = -2
f(b) = f(3) = 3² - 3 - 2 = 4
x = (af(b) - bf(a)) / (f(b) - f(a))
= (14 - 3(-2)) / (4 - (-2))
= 10 / 6
≈ 1.6667
f(x) = 1.6667² - 1.6667 - 2 ≈ -0.0556
Since f(a) _ f(x) < 0, we update b = x
Iteration 2:
a = 1, b = 1.6667
f(a) = -2
f(b) = -0.0556
x = (1_(-0.0556) - 1.6667*(-2)) / ((-0.0556) - (-2))
≈ 1.5616
f(x) = 1.5616² - 1.5616 - 2 ≈ -0.0008
Since f(a) * f(x) < 0, we update b = x
Iteration 3:
a = 1, b = 1.5616
f(a) = -2
f(b) = -0.0008
x = (1*(-0.0008) - 1.5616*(-2)) / ((-0.0008) - (-2))
≈ 1.5538
f(x) = 1.5538² - 1.5538 - 2 ≈ -0.00001
The final approximation after 3 iterations is x ≈ 1.5538.
This is very close to the actual root of the equation, which is 2 (the positive root of x² - x - 2 = 0 is (1 + √5) / 2 ≈ 1.618).
